eigene finmap implementation um schneller zu sein auf gefahr hin mehr bugs zu haben.

src/AL.v
@@ -1,13 +1,188 @@
-
-Require Import Structures.OrderedTypeEx List String.
+Require Import Structures.OrderedType Structures.OrderedTypeEx List String.
 Import ListNotations.
-Require Export FSets.FMapList.
+Require Import FSets.FMapList.
 
-Module M := FMapList.Make String_as_OT.
+Module FMap (X: OrderedType).
+  (* Include FMapList.Make X.  *)
 
-(* a.d. todo, no guarantees about overwriting but I think I only use it for constructing test data *)
-Fixpoint fromList {elt : Type} (A: list (string * elt)) : M.t elt :=
-  match A with
-  | [] => M.empty _
-  | (k, v) :: A => M.add k v (fromList A)
-  end.
+  Definition key := X.t.
+  Definition t (elt: Type) := list (key * elt)%type.
+
+  Definition empty (elt: Type) : t elt := [].
+  Fixpoint add {elt: Type} (k: key) (v: elt) (s: t elt) :=
+    match s with
+    | [] => [(k, v)]
+    | (k', v') :: s' =>
+      match X.compare k k' with
+      | LT _ => (k, v) :: s
+      | EQ _ => (k, v) :: s'
+      | GT _ => (k', v') :: add k v s'
+      end
+    end.
+  Fixpoint mem {elt: Type} (k: key) (s: t elt) :=
+    match s with
+    | [] => false
+    | (k', _) :: s' =>
+      match X.compare k k' with
+      | LT _ => false
+      | EQ _ => true
+      | GT _ => mem k s'
+      end
+    end.
+  Fixpoint find {elt: Type} (k: key) (s: t elt) : option elt :=
+    match s with
+    | [] => None
+    | (k', v) :: s' =>
+      match X.compare k k' with
+      | LT _ => None
+      | EQ _ => Some v
+      | GT _ => find k s'
+      end
+    end.
+
+  Fixpoint fold {elt A: Type} (f: key -> elt -> A -> A) (s: t elt) (state: A) : A :=
+    match s with
+    | [] => state
+    | (k, v) :: s' => fold f s' (f k v state)
+    end.
+
+  Fixpoint map {elt elt': Type} (f: elt -> elt') (s: t elt) : t elt' :=
+    match s with
+    | [] => []
+    | (k, v) :: s' => (k, f v) :: map f s'
+    end.
+
+  Fixpoint mapi {elt elt': Type} (f: key -> elt -> elt') (s: t elt) : t elt' :=
+    match s with
+    | [] => []
+    | (k, v) :: s' => (k, f k v) :: mapi f s'
+    end.
+    
+  (* a.d. todo, no guarantees about overwriting. I'm using elements -> List.map -> fromList to replace mapi since mapi seems bugged *)
+  Fixpoint fromList {elt : Type} (A: list (key * elt)) : t elt :=
+    match A with
+    | [] => empty _
+    | (k, v) :: A => add k v (fromList A)
+    end.
+End FMap. 
+
+Module SFMap := FMap String_as_OT.
+
+Require Import Arith.
+
+Module FSet (X: OrderedType).
+
+  Definition elt := X.t.
+  Definition t := list elt.
+
+  Definition empty : t := [].
+
+  Definition elements (s: t) : list elt := s.
+
+  Definition singleton (v: elt) : t := [v].
+
+  Fixpoint add (v: elt) (s: t) :=
+    match s with
+    | [] => [v]
+    | v' :: s' =>
+      match X.compare v v' with
+      | LT _ => v :: s
+      | EQ _ => s
+      | GT _ => v' :: add v s'
+      end
+    end.
+
+  Fixpoint mem (v: elt) (s: t) :=
+    match s with
+    | [] => false
+    | v' :: s' =>
+      match X.compare v v' with
+      | LT _ => false
+      | EQ _ => true
+      | GT _ => mem v s'
+      end
+    end.
+
+  Lemma size_ind {X : Type} (f : X -> nat) (P : X -> Type) :
+    (forall x, (forall y, f y < f x -> P y) -> P x) -> forall x, P x.
+  Proof.
+    intros H x. apply H.
+    induction (f x).
+    - intros y. intros []%Nat.nlt_0_r.
+    - intros y Hy. apply H.
+      intros z Hz. apply IHn.
+      apply (Nat.lt_le_trans (f z) (f y) n).
+      + apply Hz.
+      + apply lt_n_Sm_le, Hy.
+  Defined.
+
+  Fixpoint card (s: t) : nat :=
+    match s with
+    | [] => 0
+    | _ :: s' => S (card s')
+    end.
+
+  Lemma union (s0 s1: t) : t.
+    refine (size_ind (fun '(s0, s1) => card s0 + card s1) (fun _ => t) _ (s0, s1)).
+    clear s0 s1.
+    intros [s0 s1] IH.
+    destruct s0 as [|v0 s0'] eqn:H0.
+    - exact s1.
+    - destruct s1 as [|v1 s1'] eqn:H1.
+      + exact s0.
+      + refine (match X.compare v0 v1 (* as p return (X.compare v0 v1 = p -> t) *) with
+                | LT _ => _ 
+                | EQ _ => _ 
+                | GT _ => _ 
+                end (* eq_refl *)).
+        * refine (v0 :: IH (s0', v1 :: s1') _).
+          cbn. apply Nat.lt_succ_diag_r.
+        * refine (v0 :: IH (s0', s1') _).
+          cbn. rewrite Nat.add_succ_r.
+          apply (Nat.lt_trans (card s0' + card s1') (S (card s0' + card s1')) (S (S (card s0' + card s1')))).
+          apply Nat.lt_succ_diag_r. apply Nat.lt_succ_diag_r.
+        * refine (v1 :: IH (v0 :: s0', s1') _).
+          cbn. rewrite Nat.add_succ_r.
+          apply Nat.lt_succ_diag_r.
+  Defined.
+
+  Lemma intersection (s0 s1: t) : t.
+    refine (size_ind (fun '(s0, s1) => card s0 + card s1) (fun _ => t) _ (s0, s1)).
+    clear s0 s1.
+    intros [s0 s1] IH.
+    destruct s0 as [|v0 s0'] eqn:H0.
+    - exact [].
+    - destruct s1 as [|v1 s1'] eqn:H1.
+      + exact [].
+      + refine (match X.compare v0 v1 with
+                | LT _ => _
+                | EQ _ => _
+                | GT _ => _
+                end).
+        * refine (IH (s0', v1 :: s1') _).
+          cbn. apply Nat.lt_succ_diag_r.
+        * refine (v0 :: IH (s0', s1') _).
+          cbn. rewrite Nat.add_succ_r.
+          apply (Nat.lt_trans (card s0' + card s1') (S (card s0' + card s1')) (S (S (card s0' + card s1')))).
+          apply Nat.lt_succ_diag_r. apply Nat.lt_succ_diag_r.
+        * refine (IH (v0 :: s0', s1') _).
+          cbn. rewrite Nat.add_succ_r.
+          apply Nat.lt_succ_diag_r.
+  Defined.
+End FSet.
+
+Module SSet := FSet String_as_OT.
+  
+
+
+
+
+
+
+
+
+
+
+
+
+           
